chore: improve performance (#764)

AwsEncryptionSDK/runtimes/go/ImplementationFromDafny-go/awscryptographyencryptionsdksmithygenerated/to_dafny.go
@@ -159,14 +159,14 @@ func NetV4_0_0_RetryPolicy_ToDafny(nativeInput awscryptographyencryptionsdksmith
 
 func Aws_cryptography_encryptionSdk_DecryptInput_ciphertext_ToDafny(input []byte) dafny.Sequence {
 	return func() dafny.Sequence {
-		var v []interface{}
+		v := make([]interface{}, 0, len(input))
 		if input == nil {
 			return nil
 		}
 		for _, e := range input {
 			v = append(v, e)
 		}
-		return dafny.SeqOf(v...)
+		return dafny.SeqFromArray(v, false)
 	}()
 }
 
@@ -182,14 +182,14 @@ func Aws_cryptography_encryptionSdk_DecryptInput_encryptionContext_ToDafny(input
 
 func Aws_cryptography_encryptionSdk_DecryptOutput_plaintext_ToDafny(input []byte) dafny.Sequence {
 	return func() dafny.Sequence {
-		var v []interface{}
+		v := make([]interface{}, 0, len(input))
 		if input == nil {
 			return nil
 		}
 		for _, e := range input {
 			v = append(v, e)
 		}
-		return dafny.SeqOf(v...)
+		return dafny.SeqFromArray(v, false)
 	}()
 }
 
@@ -231,14 +231,14 @@ func Aws_cryptography_encryptionSdk_DecryptOutput_algorithmSuiteId_ToDafny(input
 
 func Aws_cryptography_encryptionSdk_EncryptInput_plaintext_ToDafny(input []byte) dafny.Sequence {
 	return func() dafny.Sequence {
-		var v []interface{}
+		v := make([]interface{}, 0, len(input))
 		if input == nil {
 			return nil
 		}
 		for _, e := range input {
 			v = append(v, e)
 		}
-		return dafny.SeqOf(v...)
+		return dafny.SeqFromArray(v, false)
 	}()
 }
 
@@ -288,14 +288,14 @@ func Aws_cryptography_encryptionSdk_EncryptInput_frameLength_ToDafny(input *int6
 
 func Aws_cryptography_encryptionSdk_EncryptOutput_ciphertext_ToDafny(input []byte) dafny.Sequence {
 	return func() dafny.Sequence {
-		var v []interface{}
+		v := make([]interface{}, 0, len(input))
 		if input == nil {
 			return nil
 		}
 		for _, e := range input {
 			v = append(v, e)
 		}
-		return dafny.SeqOf(v...)
+		return dafny.SeqFromArray(v, false)
 	}()
 }
 
