TestVectors/dafny/TestVectors/src/EsdkManifestOptions.dfy
@@ -7,18 +7,37 @@ module {:options "-functionSyntax:4"} EsdkManifestOptions {
   import opened Wrappers
   import Types = AwsCryptographyEncryptionSdkTypes
 
+  datatype PerfReport =
+    | ReportNone
+    | ReportIndividual
+    | ReportFinal
+    | ReportAll
+    | ReportLoop(count : nat)
+
+  predicate DoReportFinal(r : PerfReport)
+  {
+    r.ReportFinal? || r.ReportAll?
+  }
+
+  predicate DoReportIndividual(r : PerfReport)
+  {
+    r.ReportIndividual? || r.ReportAll?
+  }
+
   datatype ManifestOptions =
     | Decrypt(
         nameonly manifestPath: string,
         nameonly manifestFileName: string,
         nameonly retryPolicy: Types.NetV4_0_0_RetryPolicy,
-        nameonly testName: Option<string> := None
+        nameonly testName: Option<string> := None,
+        nameonly report: PerfReport := ReportNone
       )
     | Encrypt(
         nameonly manifestPath: string,
         nameonly manifest: string,
         nameonly decryptManifestOutput: string,
         nameonly testName: Option<string> := None,
+        nameonly report: PerfReport := ReportNone,
         nameonly legacyOutput: int := 5
       )
     | DecryptSingle(
