TestVectors/dafny/TestVectors/src/EsdkTestManifests.dfy
@@ -28,6 +28,7 @@ module {:options "-functionSyntax:4"} EsdkTestManifests {
   import EsdkManifestOptions
   import opened EsdkTestVectors
   import WriteVectors
+  import Time
 
   method StartDecryptVectors(
     op: EsdkManifestOptions.ManifestOptions
@@ -49,7 +50,7 @@ module {:options "-functionSyntax:4"} EsdkTestManifests {
       decryptManifest.jsonTests
     );
 
-    output := TestDecrypts(decryptManifest.keys, decryptVectors);
+    output := TestDecrypts(decryptManifest.keys, decryptVectors, op.report);
   }
 
   predicate TestDecryptVector?(v: EsdkDecryptTestVector)
@@ -59,7 +60,8 @@ module {:options "-functionSyntax:4"} EsdkTestManifests {
 
   method TestDecrypts(
     keys: KeyVectors.KeyVectorsClient,
-    vectors: seq<EsdkDecryptTestVector>
+    vectors: seq<EsdkDecryptTestVector>,
+    report: EsdkManifestOptions.PerfReport
   )
     returns (manifest: Result<seq<BoundedInts.byte>, string>)
     requires keys.ValidState()
@@ -70,12 +72,18 @@ module {:options "-functionSyntax:4"} EsdkTestManifests {
 
     var hasFailure := false;
     var skipped := 0;
+    var time := Time.GetAbsoluteTime();
 
     for i := 0 to |vectors|
     {
       var vector := vectors[i];
       if TestDecryptVector?(vector) {
-        var pass := EsdkTestVectors.TestDecrypt(keys, vector);
+        var itime := Time.GetAbsoluteTime();
+        var pass := EsdkTestVectors.TestDecrypt(keys, vector, report);
+        if EsdkManifestOptions.DoReportIndividual(report) {
+          var elapsed := Time.TimeSince(itime);
+          Time.PrintTimeLong(elapsed, "Decrypt " + vector.id, Some(LogFileName()));
+        }
         if !pass {
           hasFailure := true;
         }
@@ -83,8 +91,12 @@ module {:options "-functionSyntax:4"} EsdkTestManifests {
         skipped := skipped + 1;
         print "\nSKIP===> ", vector.id, "\n";
       }
-
     }
+    if EsdkManifestOptions.DoReportFinal(report) {
+      var elapsed := Time.TimeSince(time);
+      Time.PrintTimeLong(elapsed, "TestDecrypts ESDK", Some(LogFileName()));
+    }
+
     print "\n=================== Completed ", |vectors|, " Decrypt Tests =================== \n\n";
 
     if 0 < skipped {
@@ -92,6 +104,15 @@ module {:options "-functionSyntax:4"} EsdkTestManifests {
     }
 
     manifest := if !hasFailure then Success([]) else Failure("Test Vectors failed, see errors above.\n");
+  }
+
+  method GetRandom(n : mplTypes.PositiveInteger) returns (out : seq<uint8>)
+  {
+    var p :- expect AtomicPrimitives.AtomicPrimitives();
+    out :- expect p.GenerateRandomBytes(
+      AtomicPrimitives.Types.GenerateRandomBytesInput(
+        length := n
+      ));
   }
 
   method {:vcs_split_on_every_assert} StartEncryptVectors(
@@ -111,15 +132,11 @@ module {:options "-functionSyntax:4"} EsdkTestManifests {
       encryptManifest.jsonTests
     );
 
-    var p :- expect AtomicPrimitives.AtomicPrimitives();
     var plaintext := map[];
     for i := 0 to |encryptManifest.plaintext|
     {
       var (name, length) := encryptManifest.plaintext[i];
-      var data :- expect p.GenerateRandomBytes(
-        AtomicPrimitives.Types.GenerateRandomBytesInput(
-          length := length
-        ));
+      var data := GetRandom(length);
       // Write the plaintext to disk.
       print op.decryptManifestOutput + plaintextPathRoot + name, "\n\n";
       var _ :- WriteVectorsFile(op.decryptManifestOutput + plaintextPathRoot + name, data);
@@ -128,7 +145,7 @@ module {:options "-functionSyntax:4"} EsdkTestManifests {
 
     var encryptTests? := ToEncryptTests(encryptManifest.keys, encryptVectors);
     var encryptTests :- encryptTests?.MapFailure((e: KeyVectorsTypes.Error) => var _ := MplVectorPrintErr(e); "Cmm failure");
-    var decryptVectors :- TestEncrypts(plaintext, encryptManifest.keys, encryptTests);
+    var decryptVectors :- TestEncrypts(plaintext, encryptManifest.keys, encryptTests, op.report);
 
     var _ :- WriteVectors.WriteDecryptManifest(op, encryptManifest.keys, decryptVectors);
 
@@ -167,7 +184,8 @@ module {:options "-functionSyntax:4"} EsdkTestManifests {
   method TestEncrypts(
     plaintexts: map<string, seq<uint8>>,
     keys: KeyVectors.KeyVectorsClient,
-    tests: seq<EsdkTestVectors.EncryptTest>
+    tests: seq<EsdkTestVectors.EncryptTest>,
+    report: EsdkManifestOptions.PerfReport
   )
     returns (manifest: Result<seq<EsdkDecryptTestVector>, string>)
     requires keys.ValidState()
@@ -183,6 +201,7 @@ module {:options "-functionSyntax:4"} EsdkTestManifests {
     var hasFailure := false;
     var decryptVectors := [];
     var skipped := [];
+    var time := Time.GetAbsoluteTime();
 
     for i := 0 to |tests|
       invariant forall t <- tests ::
@@ -199,7 +218,13 @@ module {:options "-functionSyntax:4"} EsdkTestManifests {
           && test.vector.algorithmSuiteId.value.id.ESDK?,
           "Vector is using an algorithm suite other than ESDK"
         );
-        var pass :- EsdkTestVectors.TestEncrypt(plaintexts, keys, test);
+        var itime := Time.GetAbsoluteTime();
+        var pass :- EsdkTestVectors.TestEncrypt(plaintexts, keys, test, report);
+        if EsdkManifestOptions.DoReportIndividual(report) {
+          var elapsed := Time.TimeSince(itime);
+          Time.PrintTimeLong(elapsed, "Encrypt " + test.vector.id.UnwrapOr("unknown"), Some(LogFileName()));
+        }
+
         if !pass.output {
           hasFailure := true;
         } else if pass.vector.Some? {
@@ -209,6 +234,10 @@ module {:options "-functionSyntax:4"} EsdkTestManifests {
         skipped := skipped + [test.vector.id.value + "\n"];
         print "\nSKIP===> ", test.vector.id.value, "\n";
       }
+    }
+    if EsdkManifestOptions.DoReportFinal(report) {
+      var elapsed := Time.TimeSince(time);
+      Time.PrintTimeLong(elapsed, "TestEncrypts ESDK", Some(LogFileName()));
     }
     print "\n=================== Completed ", |tests|, " Encrypt Tests =================== \n\n";
 
